Some progress on the proof of RST.Vector

ulib/LowStar.RST.Vector.fst
@@ -3,61 +3,134 @@ module LowStar.RST.Vector
 
 open LowStar.RST
 module HS = FStar.HyperStack
+module HST = FStar.HyperStack.ST
 module A = LowStar.RST.Array
 module Arr = LowStar.Array
 module P = LowStar.RST.Pointer
 module U32 = FStar.UInt32
-
+module L = LowStar.RST.Loops
 module S = FStar.Seq
+module Perm = LowStar.Permissions
 #set-options "--max_fuel 0 --max_ifuel 0"
 
 noeq
 type vector_s (a: Type0) =
 | Vector:
     len:U32.t -> // number of elements in the vector
-    max:U32.t -> // capacity r
+    max:U32.t -> // capacity
     arr:A.array a ->
     vector_s a
 
 let vector (a: Type0) = P.pointer (vector_s a)
+
+let hget_arr (h: HS.mem) (#a: Type0) (v:vector a) : GTot (A.array a) =
+  (Seq.index (A.as_seq h v) 0).arr
+let hget_len (h: HS.mem) (#a: Type0) (v:vector a) : GTot U32.t = (Seq.index (A.as_seq h v) 0).len
+let hget_max (h: HS.mem) (#a: Type0) (v:vector a) : GTot U32.t = (Seq.index (A.as_seq h v) 0).max
+let hget_perm (h : HS.mem) (#a: Type0) (v:vector a)
+  : GTot (Ghost.erased LowStar.Permissions.permission) =
+  Ghost.hide (A.get_perm h (hget_arr h v) 0)
+let hget_seq (h: HS.mem) (#a: Type0) (v:vector a) : GTot (Seq.seq a) =
+  A.as_seq h (hget_arr h v)
+let hget_arr_r (h: HS.mem) (#a: Type0) (v:vector a) : GTot resource =
+  A.array_resource (hget_arr h v)
 
 let vector_view (#a : Type0) (v : vector a) : Tot (view (vector_view_t a)) =
   let v_ptr_r : resource = P.ptr_resource v in
   reveal_view ();
   P.reveal_ptr ();
   A.reveal_array ();
-  let get_arr (h: HS.mem) : GTot (A.array a) = (Seq.index (A.as_seq h v) 0).arr in
-  let get_len (h: HS.mem) : GTot U32.t = (Seq.index (A.as_seq h v) 0).len in
-  let get_max (h: HS.mem) : GTot U32.t = (Seq.index (A.as_seq h v) 0).max in
-  let get_perm (h : HS.mem) : GTot (Ghost.erased LowStar.Permissions.permission) =
-    Ghost.hide (A.get_perm h (get_arr h) 0)
-  in
-  let get_seq (h: HS.mem) : GTot (Seq.seq a) =
-    A.as_seq h (get_arr h)
-  in
-  let v_arr_r (h: HS.mem) : GTot resource = A.array_resource (get_arr h) in
-  let fp (h: HS.mem) =
-     (A.loc_array v)
+
+  let fp_r (h: HS.mem) =
+    (as_loc (fp (P.ptr_resource v)) h)
     `A.loc_union`
-    (A.loc_array (Seq.index (A.as_seq h v) 0).arr)
+    (as_loc (fp (A.array_resource (hget_arr h v))) h)
   in
-  let inv (h: HS.mem) : prop =
-    inv v_ptr_r h /\ inv (v_arr_r h) h /\
-    U32.v (get_len h) <= U32.v (get_max h) /\
-    U32.v (get_len h) >= 0
+  let inv_r (h: HS.mem) : prop =
+    inv v_ptr_r h /\ inv (hget_arr_r h v) h /\
+    (as_loc (fp (P.ptr_resource v)) h) `A.loc_disjoint`
+      (as_loc (fp (A.array_resource (hget_arr h v))) h) /\
+    A.length (hget_arr h v) = hget_max h v /\
+    U32.v (hget_len h v) <= U32.v (hget_max h v) /\
+    U32.v (hget_len h v) >= 0 /\
+    Ghost.reveal (hget_perm h v) = A.get_perm h v 0 /\
+    A.freeable (hget_arr h v)
   in
-  let sel (h: HS.mem) : GTot (vector_view_t a) =
+  let sel_r (h: HS.mem) : GTot (vector_view_t a) =
+    let len = U32.v  (hget_len h v) in
+    let correct_len = if len >= 0 && len <= S.length (hget_seq h v) then len else 0 in
     {
-      v_capacity = get_max h;
-      v_arr = get_seq h;
-      v_perm = get_perm h;
+      v_capacity = hget_max h v;
+      v_arr = S.slice (hget_seq h v) 0 correct_len;
+      v_perm = hget_perm h v;
     }
   in
-  { fp; inv; sel }
+  { fp = fp_r ; inv = inv_r; sel = sel_r }
 
 
 let create #a init max =
-  admit()
+  (**) reveal_empty_resource ();
+  (**) reveal_rst_inv ();
+  (**) reveal_view ();
+  (**) P.reveal_ptr ();
+  (**) A.reveal_array ();
+  (**) reveal_modifies ();
+  let contents = A.alloc init max in
+  let v = Vector 0ul max contents in
+  let ptr = P.ptr_alloc v in
+  ptr
+
+#set-options "--z3rlimit 20"
 
 let push #a v x =
-  admit()
+  (**) reveal_empty_resource ();
+  (**) reveal_rst_inv ();
+  (**) reveal_view ();
+  (**) reveal_star ();
+  (**) P.reveal_ptr ();
+  (**) A.reveal_array ();
+  (**) reveal_modifies ();
+  let v_record = P.ptr_read v in
+  let max = v_record.max in
+  let len = v_record.len in
+  (**) let h0 = HST.get () in
+  if U32.(len <^ max) then begin
+    A.upd v_record.arr len x;
+    P.ptr_write v (Vector U32.(v_record.len +^ 1ul) v_record.max v_record.arr);
+    (**) let h1 = HST.get () in
+    (**) assert(
+    (**)   S.slice (hget_seq h1 v) 0 (U32.v len + 1) `S.equal`
+    (**)     S.snoc (S.slice (hget_seq h0 v) 0 (U32.v len)) x
+    (**) )
+  end else begin
+    let max_uint32 = UInt32.uint_to_t (UInt.max_int 32) in
+    let new_contents_lenght =
+      if U32.(max >^ max_uint32 /^ 2ul) then
+        max_uint32
+      else
+        U32.(2ul *^ max)
+    in
+    let new_contents = A.alloc x new_contents_lenght in
+    (**) let h1 = HST.get () in
+    (**) let sub_new = LowStar.Array.sub new_contents 0ul len in
+    (**) reveal_star_inv (A.array_resource sub_new) (A.array_resource v_record.arr) h1;
+    (**) assert(inv (A.array_resource v_record.arr) h1);
+    (**) assume(inv (A.array_resource sub_new) h1);
+    (**) assume(A.fresh_loc (A.loc_array new_contents) h0 h1);
+    (**) assume(A.loc_disjoint (A.loc_array sub_new) (A.loc_array v_record.arr));
+    (**) assume(rst_inv (A.array_resource sub_new <*> A.array_resource v_record.arr) h1);
+    A.copy sub_new v_record.arr;
+    (**) let h2 = HST.get () in
+    A.free v_record.arr;
+    (**) let h3 = HST.get () in
+    let new_v_record = Vector len max new_contents in
+    (**) assume(inv (P.ptr_resource v) h3);
+    (**) assume(rst_inv (P.ptr_resource v) h3);
+    (**) assume(Perm.allows_write (A.get_perm h3 v 0));
+    P.ptr_write v new_v_record;
+    (**) let h4 = HST.get () in
+    (**) assume(inv (vector_resource v) h4);
+    (**) assume(rst_inv (vector_resource v) h4);
+    (**) assume(A.modifies (as_loc (fp (vector_resource v)) h0) h0 h4);
+    (**) assume(frame_usedness_preservation (as_loc (fp ((vector_resource v))) h0) (as_loc (fp ((vector_resource v))) h4) h0 h4)
+  end
